Remove StampedMap from spec

Spec/MapSpec.s.dfy
@@ -4,35 +4,60 @@
 include "../lib/Base/KeyType.s.dfy"
 include "../lib/Base/SequencesLite.s.dfy"
 include "Message.s.dfy"
-include "StampedMap.s.dfy"
 include "AtomicStateMachine.s.dfy"
 include "CrashTolerant.s.dfy"
+
+module FullKMMapMod {
+  import opened ValueMessage
+  import opened KeyType
+  // Defines a fully-populated Key-Message imap
+
+  predicate AnyKey<K>(k: K) { true }
+  predicate Defined(kvm: imap<Key, Message>, k: Key) {
+    k in kvm && kvm[k].Define?
+  }
+  predicate KMMapIsFull(kvm: imap<Key, Message>) {
+    forall k | AnyKey(k) :: Defined(kvm, k)
+  }
+  function EmptyKMMap() : imap<Key, Message>
+    ensures KMMapIsFull(EmptyKMMap())
+  {
+    imap k | AnyKey(k) :: DefaultMessage()
+  }
+
+  // Dafny demands a compilable witness for FullKMMap, but also doesn't
+  // compile imaps. Lucky we're in a .s file so I can just lie with an
+  // axiom. This makes me feel uncomfortable.
+  function method Witness() : imap<Key,Message> ensures Witness() == EmptyKMMap()
+  type FullKMMap = ikv: imap<Key,Message> | KMMapIsFull(ikv) witness Witness()
+}
 
 module MapSpecMod refines AtomicStateMachineMod {
   import opened ValueMessage
   import opened KeyType
-  import StampedMapMod
+  import opened FullKMMapMod
 
   // UI
   datatype Input = GetInput(key: Key) | PutInput(key: Key, value: Value) | NoopInput
   datatype Output = GetOutput(value: Value) | PutOutput | NoopOutput
 
   // State machine
-  datatype Variables = Variables(smap: StampedMapMod.StampedMap)
+  datatype Variables = Variables(kmmap: FullKMMap)
 
   function InitState() : Variables {
-    Variables(StampedMapMod.Empty())
+    Variables(EmptyKMMap())
   }
 
   predicate Query(v: Variables, v': Variables, key: Key, value: Value)
   {
-    && value == v.smap.mi[key].value
+    && assert AnyKey(key);
+    && value == v.kmmap[key].value
     && v' == v
   }
 
   predicate Put(v: Variables, v': Variables, key: Key, value: Value)
   {
-    && v' == v.(smap := v.smap.Put(key, Define(value)))
+    && v' == v.(kmmap := v.kmmap[key := Define(value)])
   }
 
   predicate Next(v: Variables, v': Variables, input: Input, out: Output)
