Splinter/BranchTreeStack.i.dfy
@@ -6,7 +6,7 @@ include "AllocationTableMachine.i.dfy"
 include "CoordinationLayer/MsgHistory.i.dfy"
 include "BranchTree.i.dfy"
 include "../Spec/Message.s.dfy"
-include "../Spec/StampedMap.s.dfy"
+include "CoordinationLayer/StampedMap.i.dfy"
 include "BranchTreeInterp.i.dfy"
 include "../lib/Base/Sequences.i.dfy"
 
