Splinter/SplinterTreeInterp.i.dfy
@@ -9,7 +9,7 @@ include "CoordinationLayer/MsgHistory.i.dfy"
 include "SplinterTree.i.dfy"
 include "BranchTreeInterp.i.dfy"
 include "../Spec/Message.s.dfy"
-include "../Spec/StampedMap.s.dfy"
+include "CoordinationLayer/StampedMap.i.dfy"
 include "../lib/Base/mathematics.i.dfy"
 
 // interpretation for the SplinterTree Implementation
